refactored bpar case in Impl_vm

src/Impl_vm.v
@@ -38,6 +38,12 @@ Fixpoint build_comp (t:AnnoTerm): VM unit :=
     p <- get_pl ;;
     pr <- split_evm x sp1 sp2 e p ;;
     let '(e1,e2) := pr in
+    let loc_e1 := fst (range t1) in
+    let loc_e1' := fst (range t1) in
+    let loc_e2 := fst (range t2) in
+    let loc_e2':= fst (range t2) in
+    put_store_at loc_e1 e1 ;;
+    put_store_at loc_e2 e2 ;;
     (*
     let res1 := parallel_att_vm_thread t1 e in
     (* TODO: change this to a monadic function that consults an environment that is aware of the presence (or absence) of parallel avm threads.  Put initial evidence in store, let environment run the parallel thread and place result evidence, then query for result evidence here. *)
@@ -50,12 +56,10 @@ Fixpoint build_comp (t:AnnoTerm): VM unit :=
     put_store loc2 res2 ;;
     add_tracem (shuffled_events el1 el2) ;; *)
 
-    runParThreads t1 t2 p e1 e2 ;;
-    let loc1 := fst (range t1) in
-    let loc2 := fst (range t2) in
+    runParThreads t1 t2 p loc_e1 loc_e1' loc_e2 loc_e2'  ;;
        
-    e1r <- get_store_at loc1 ;;
-    e2r <- get_store_at loc2 ;;
+    e1r <- get_store_at loc_e1' ;;
+    e2r <- get_store_at loc_e2' ;;
     put_ev (ppc e1r e2r) ;;
     add_tracem [Term.join (Nat.pred y) p]
   end.
